theories/syntax.v
@@ -3,10 +3,6 @@ Import ListNotations.
 
 From RichWasm.syntax Require Export module rw.
 
-Definition primitive_rep_eq_dec (ι1 ι2 : primitive_rep) : {ι1 = ι2} + {ι1 <> ι2}.
-  decide equality.
-Defined.
-
 Fixpoint flatten_func_type (ϕ : function_type) : list kind * list type * list type :=
   match ϕ with
   | MonoFunT τs1 τs2 => ([], τs1, τs2)
